Expose contiguous nature of Var/Lit

Valaig/Aig/Refs.lean
@@ -8,18 +8,23 @@ namespace Valaig
 
 /--
 Variable: a reference to a node in an Aig based on its index.
+
+These have contiguous indices, with the constant variable (taken to be `false` if not inverted)
+represented by index 0. Where possible, users should prefer dealing directly with `Var` rather
+than accessing the underlying index with `Var.idx`. The primary use for direct access to the index
+is for indexing into contiguous memory (`Array`s).
 -/
 structure Var where
   ofIdx ::
     idx : Nat
 
 namespace Var
+variable {var : Var}
 
 deriving instance DecidableEq, Repr, Inhabited, BEq, ReflBEq, LawfulBEq for Var
 
 instance : EquivBEq Var := by constructor
 
-@[local grind =_]
 theorem ext_idx (var var' : Var) :
     var = var' ↔ var.idx = var'.idx := by
   grind only [Var]
@@ -31,7 +36,6 @@ instance : LE Var where le := (·.idx ≤ ·.idx)
 instance : DecidableLE Var := fun a b =>
   decidable_of_bool (a.idx ≤ b.idx) (by simp +instances [Var.instLE])
 
-@[local grind =]
 theorem le_idx (var var' : Var) :
     var ≤ var' ↔ var.idx ≤ var'.idx := by
   simp +instances [instLE]
@@ -39,20 +43,33 @@ theorem le_idx (var var' : Var) :
 instance : Std.IsLinearOrder Var := by
   apply Std.IsLinearOrder.of_le
   <;> constructor
-  <;> grind
+  <;> grind [ext_idx, le_idx]
 
 instance : LT Var where lt := (·.idx < ·.idx)
 instance : DecidableLT Var := fun a b =>
   decidable_of_bool (a.idx < b.idx) (by simp +instances [Var.instLT])
 
-@[local grind =]
 theorem lt_idx (var var' : Var) :
     var < var' ↔ var.idx < var'.idx := by
   simp +instances [instLT]
 
+grind_pattern le_idx => var.idx, var'.idx, var ≤ var'
+grind_pattern le_idx => var.idx, var'.idx, var > var'
+grind_pattern lt_idx => var.idx, var'.idx, var < var'
+grind_pattern lt_idx => var.idx, var'.idx, var ≥ var'
+
 instance : Std.LawfulOrderLT Var := by
   apply Std.LawfulOrderLT.of_le
-  grind
+  grind [lt_idx]
+
+instance : WellFoundedRelation Var where
+  rel := (· < ·)
+  wf := by
+    constructor
+    have {var : Var} : Acc (· < ·) var := by
+      induction h : var.idx generalizing var
+      <;> grind [Acc, lt_idx]
+    apply this
 
 instance : Min Var := minOfLe
 
@@ -72,47 +89,61 @@ instance : Std.LawfulOrderMax Var := by
 instance : Hashable Var where hash := (hash ·.idx)
 instance : LawfulHashable Var where hash_eq := by simp
 
-instance : WellFoundedRelation Var where
-  rel := (· < ·)
-  wf := by
-    constructor
-    have {var : Var} : Acc (· < ·) var := by
-      induction h : var.idx generalizing var
-      <;> grind [Acc]
-    apply this
-
 @[inline]
 def constant : Var :=
   .ofIdx 0
 
-theorem constant_idx_eq_zero :
+@[simp, grind =]
+theorem idx_constant :
     constant.idx = 0 := by
   simp [constant]
 
-@[inline]
-def offset (v : Var) (n : Nat) : Var :=
-  .ofIdx (v.idx + n)
+theorem eq_constant_iff_idx_eq_zero :
+    var = constant ↔ var.idx = 0 := by
+  grind [Var.ext_idx]
 
 @[inline]
-def next (v : Var) : Var :=
-  v.offset 1
+def offset (var : Var) (n : Nat) : Var :=
+  .ofIdx (var.idx + n)
+
+@[simp, grind =]
+theorem idx_offset {n : Nat} :
+    (var.offset n).idx = var.idx + n := by
+  simp [offset]
+
+/--
+Adding a `Nat` to a `Var` increments the `Var`'s index.
+This is defined in terms of `offset` to hide the implementation details.
+-/
+@[inline, expose, reducible, grind unfold]
+instance : HAdd Var Nat Var where
+  hAdd (var : Var) (n : Nat) :=
+    var.offset n
+
+@[simp]
+theorem add_eq {n : Nat} :
+    var + n = var.offset n := by
+  rfl
 
 @[inline]
 def ofRef {α} [DecidableEq α] [Hashable α] {aig : Std.Sat.AIG α} (ref : aig.Ref) : Var :=
   .ofIdx ref.gate
 
-@[simp, grind! .]
-theorem ofRef_idx {α} [DecidableEq α] [Hashable α] {aig : Std.Sat.AIG α} (ref : aig.Ref) :
+@[simp, grind =]
+theorem idx_ofRef {α} [DecidableEq α] [Hashable α] {aig : Std.Sat.AIG α} (ref : aig.Ref) :
     (ofRef ref).idx = ref.gate := by
   simp only [ofRef]
 
 end Var
 
 /--
-Literal: an invertible reference to a `Variable` in an `Aig`.
+Literal: an invertible reference to a `Var` in an `Aig`.
+
+These are represented by storing the inversion in the least significant bit and the variable
+left-shifted by one in the higher bits. Although this detail is exposed for use with contiguous
+containers, care should be taken to avoid relying on it whenever possible.
 -/
 structure Lit where
-  -- TODO: It would be nice to mark this constructor private but the parser uses it currently.
   ofIdx ::
     idx : Nat
 
@@ -134,8 +165,23 @@ instance : LawfulHashable Lit where hash_eq := by simp
 Returns a literal referencing a variable which is optionally inverted.
 -/
 @[inline]
-def mk (v : Var) (invert : Bool := false) : Lit :=
-  .ofIdx <| v.idx <<< 1 ||| invert.toNat
+def mk (var : Var) (invert : Bool := false) : Lit :=
+  .ofIdx <| var.idx <<< 1 ||| invert.toNat
+
+@[simp]
+theorem idx_mk {invert : Bool} :
+    (mk var invert).idx = var.idx * 2 + invert.toNat := by
+  have := @Nat.two_pow_add_eq_or_of_lt 1
+  grind only [Bool.toNat_lt, Nat.shiftLeft_eq, mk]
+
+@[grind =]
+theorem idx_mk_cases {invert : Bool} :
+    (mk var invert).idx =
+    if invert then
+      var.idx * 2 + 1
+    else
+      var.idx * 2 := by
+  grind [idx_mk]
 
 /--
 Returns the variable referenced by a literal.
@@ -146,13 +192,23 @@ def var (l : Lit) : Var :=
   .ofIdx <| l.idx / 2
 
 @[simp, grind =]
-theorem mk_var (var : Var) (invert: Bool) :
+theorem var_mk (var : Var) (invert : Bool) :
     (Lit.mk var invert).var = var := by
   have : invert.toNat / 2 = 0 := by
     have := Bool.toNat_le invert
     omega
   rw [Lit.var, mk, Nat.or_div_two, this, Nat.or_zero, Nat.shiftLeft_eq, Nat.mul_div_cancel]
   omega
+
+@[simp]
+theorem idx_lt_of_var_lt {lit' : Lit} (lt : lit.var < lit'.var) :
+    lit.idx < lit'.idx := by
+  grind only [var, Var.lt_idx]
+
+grind_pattern idx_lt_of_var_lt => lit.idx, lit.var < lit'.var
+grind_pattern idx_lt_of_var_lt => lit'.idx, lit.var < lit'.var
+grind_pattern idx_lt_of_var_lt => lit.idx, lit.var ≥ lit'.var
+grind_pattern idx_lt_of_var_lt => lit'.idx, lit.var ≥ lit'.var
 
 /--
 Returns the whether the literal is inverted.
@@ -167,13 +223,13 @@ instance {l : Lit} : Decidable l.inverted :=
   decidable_of_iff _ this
 
 @[simp, grind .]
-theorem mk_inverted (var : Var) (invert : Bool) :
+theorem inverted_mk (var : Var) (invert : Bool) :
     (Lit.mk var invert).inverted = invert := by
   unfold mk inverted
   by_cases invert <;> simp_all
 
 @[simp, grind =, local grind! .]
-theorem mk_eq_self :
+theorem mk_self_eq :
     Lit.mk lit.var lit.inverted = lit := by
   rw [mk, var, ext_idx]
   by_cases h : lit.inverted
@@ -182,7 +238,7 @@ theorem mk_eq_self :
 
 theorem ext {lit lit' : Lit} :
     lit = lit' ↔ (lit.var = lit'.var ∧ lit.inverted = lit'.inverted) := by
-  grind only [mk_eq_self]
+  grind only [mk_self_eq]
 
 @[simp, grind =]
 theorem mk_ext {var var' : Var} {invert invert' : Bool} :
@@ -197,7 +253,7 @@ def constant (value : Bool) : Lit :=
   .ofIdx value.toNat
 
 @[simp, grind =]
-theorem constant_def :
+theorem constant_eq :
     constant invert = mk .constant invert := by
   simp [constant, mk, Var.constant]
 
@@ -210,17 +266,9 @@ def false : Lit :=
   .ofIdx 0
 
 @[simp, grind =]
-theorem false_def :
+theorem false_eq :
     false = constant .false := by
   simp [constant, false]
-
-/--
-Sometimes useful for induction. TODO: How much do we want to expose these?
--/
-theorem idx_lt_of_var_lt {lit' : Lit} (lt : lit.var < lit'.var) :
-    lit.idx < lit'.idx := by
-  simp +instances [var, Var.instLT] at lt
-  omega
 
 /--
 The (single) true literal.
@@ -231,7 +279,7 @@ def true : Lit :=
   .ofIdx 1
 
 @[simp, grind =]
-theorem true_def :
+theorem true_eq :
     true = constant .true := by
   simp [constant, true]
 
@@ -245,25 +293,25 @@ def isConstant (l : Lit) : Prop :=
 @[inline]
 instance {l : Lit} : Decidable l.isConstant :=
   have : l.idx < 2 ↔ l.isConstant := by
-    simp [isConstant, Var.constant, Var.ext_idx, var]
+    simp [isConstant, Var.constant, var]
   decidable_of_iff _ this
 
 @[simp, grind =]
-theorem isConstant_def :
+theorem isConstant_eq :
     lit.isConstant ↔ lit.var = .constant := by
   rw [isConstant]
 
 @[simp]
-theorem true_isConstant :
+theorem isConstant_true :
     true.isConstant := by
   simp [isConstant]
 
 @[simp]
-theorem false_isConstant :
+theorem isConstant_false :
     false.isConstant := by
   simp [isConstant]
 
-theorem isConstant_iff_false_or_true :
+theorem isConstant_iff_eq_false_or_eq_true :
     lit.isConstant ↔ lit = false ∨ lit = true := by
   grind
 
@@ -281,24 +329,24 @@ def asConstant (l : Lit) : Option Bool :=
     none
 
 @[simp]
-theorem asConstant_false :
+theorem asConstant_false_iff :
     lit.asConstant = some .false ↔ lit = .false := by
   simp [asConstant, Var.constant, ext_idx, var, mk, UInt8.ofNat_eq_iff_mod_eq_toNat]
   grind only
 
 @[simp]
-theorem asConstant_true :
+theorem asConstant_true_iff :
     lit.asConstant = some .true ↔ lit = .true := by
   simp [asConstant, Var.constant, ext_idx, var, mk, UInt8.ofNat_eq_iff_mod_eq_toNat]
   grind only
 
 @[simp]
-theorem asConstant_none :
+theorem asConstant_none_iff :
     lit.asConstant = none ↔ ¬lit.isConstant:= by
   simp [asConstant]
 
 @[grind =]
-theorem asConstant_def :
+theorem asConstant_eq :
     lit.asConstant =
     if lit = false then
       some .false
@@ -306,7 +354,7 @@ theorem asConstant_def :
       some .true
     else
       none := by
-  grind [asConstant_false, asConstant_true, asConstant_none]
+  grind [asConstant_false_iff, asConstant_true_iff, asConstant_none_iff]
 
 /--
 Optionally inverts the polarity of a literal.
@@ -327,7 +375,7 @@ theorem invert_true :
   simp [var, inverted, Nat.xor_div_two]
 
 @[simp, grind =]
-theorem invert_def {doInvert : Bool} :
+theorem invert_eq {doInvert : Bool} :
     lit.invert doInvert = mk lit.var (lit.inverted ≠ doInvert) := by
   simp; grind
 
@@ -341,7 +389,7 @@ def strip (l : Lit) : Lit :=
   .ofIdx <| l.idx ^^^ (l.idx &&& 1)
 
 @[simp, grind =]
-theorem strip_def :
+theorem strip_eq :
     lit.strip = mk lit.var .false := by
   rw [strip, ext] <;> simp
   simp [var, inverted, Nat.xor_div_two]
@@ -355,7 +403,7 @@ def ofFanin (fi : Std.Sat.AIG.Fanin) : Lit :=
 -- Should we prove this by showing individually that gate and invert map?
 open Std.Sat.AIG in
 @[simp, grind =]
-theorem ofFanin_def (fi : Fanin) :
+theorem ofFanin_eq (fi : Fanin) :
     ofFanin fi = mk (.ofIdx fi.gate) fi.invert := by
   rw [ext]
   unfold ofFanin Fanin.gate Fanin.invert mk var inverted
@@ -403,7 +451,7 @@ def ofRef (ref : aig.Ref) : Lit :=
   mk (.ofRef ref) ref.invert
 
 @[simp, grind =]
-theorem ofRef_def (ref : aig.Ref) :
+theorem ofRef_eq (ref : aig.Ref) :
     ofRef ref = mk (.ofRef ref) ref.invert := by
   rw [ofRef]
 
@@ -416,8 +464,8 @@ theorem toRef_gate (h : lit.var.idx < aig.decls.size) :
     (toRef lit h).gate = lit.var.idx := by
   rw [toRef]
 
-@[simp, grind =]
-theorem toRef_invert_eq_inverted (h : lit.var.idx < aig.decls.size) :
+@[simp]
+theorem toRef_invert_eq_true (h : lit.var.idx < aig.decls.size) :
     (toRef lit h).invert = lit.inverted := by
   simp [toRef]
 
@@ -430,6 +478,6 @@ end
 
 end Lit
 
-@[inline, simp]
-abbrev Var.toLit (v : Var) (invert : Bool := false) : Lit :=
-  .mk v invert
+@[inline, expose, reducible, simp, grind unfold]
+def Var.toLit (var : Var) (invert : Bool := false) : Lit :=
+  .mk var invert
